feat: rewrite the tactic using `simp` as the basis.

src/Lean/Meta/Tactic/AC/Main.lean
@@ -13,7 +13,6 @@ open Lean.Data.AC
 open Lean.Elab.Tactic
 
 abbrev ACExpr := Lean.Data.AC.Expr
-open Lean.Data.AC.Expr
 
 structure PreContext where
   id : Nat
@@ -23,44 +22,15 @@ structure PreContext where
   idem : Option Expr
   deriving Inhabited
 
-instance : ContextInformation (Std.HashMap Nat (Option Expr) × PreContext) where
-  isComm ctx := ctx.2.comm.isSome
-  isIdem ctx := ctx.2.idem.isSome
-  isNeutral ctx x := ctx.1.find? x |>.bind id |>.isSome
+instance : ContextInformation (PreContext × Array Bool) where
+  isComm ctx := ctx.1.comm.isSome
+  isIdem ctx := ctx.1.idem.isSome
+  isNeutral ctx x := ctx.2[x]
 
 instance : EvalInformation PreContext ACExpr where
-  arbitrary _ := var 0
-  evalOp _ := op
-  evalVar _ x := var x
-
-structure ACNormContext where
-  preContexts : ExprMap (Option PreContext)
-  preContextsReverse : Array PreContext
-  exprIds : ExprMap Nat
-  exprIdsReverse : Array Expr
-  neutrals : Std.HashMap (Nat × Nat) (Option Lean.Expr)
-
-def emptyACNormContext : ACNormContext :=
-  { preContexts := Std.HashMap.empty,
-    exprIds := Std.HashMap.empty,
-    exprIdsReverse := #[]
-    preContextsReverse := #[],
-    neutrals := Std.HashMap.empty }
-
-abbrev M α := StateT ACNormContext MetaM α
-
-def lazyCache
-  (lookup : ACNormContext → α → Option β)
-  (insert : ACNormContext → α → β → ACNormContext)
-  (create : ACNormContext → α → MetaM β)
-  (a : α) : M β := do
-  let state ← get
-  if let some b := lookup state a then
-    return b
-  else
-    let b ← create state a
-    set $ insert state a b
-    return b
+  arbitrary _ := Data.AC.Expr.var 0
+  evalOp _ := Data.AC.Expr.op
+  evalVar _ x := Data.AC.Expr.var x
 
 def getInstance (cls : Name) (exprs : Array Expr) : MetaM (Option Expr) := do
   try
@@ -72,183 +42,74 @@ def getInstance (cls : Name) (exprs : Array Expr) : MetaM (Option Expr) := do
   catch
   | _ => return none
 
-def preContextCache : Expr → M (Option PreContext) :=
-  lazyCache
-    (fun ctx => ctx.preContexts.find?)
-    (fun ctx a b => { ctx with
-      preContexts := ctx.preContexts.insert a b,
-      preContextsReverse := if let some b := b then ctx.preContextsReverse.push b else ctx.preContextsReverse })
-    fun ctx expr => do
-    if let some assoc := ←getInstance ``IsAssociative #[expr] then
-      return some
-        { assoc,
-          op := expr
-          id := ctx.preContextsReverse.size
-          comm := ←getInstance ``IsCommutative #[expr]
-          idem := ←getInstance ``IsIdempotent #[expr] }
+def preContext (expr : Expr) : MetaM (Option PreContext) := do
+  if let some assoc := ←getInstance ``IsAssociative #[expr] then
+    return some
+      { assoc,
+        op := expr
+        id := 0
+        comm := ←getInstance ``IsCommutative #[expr]
+        idem := ←getInstance ``IsIdempotent #[expr] }
 
-    return none
+  return none
 
-def exprId : Expr → M Nat :=
-  lazyCache
-    (fun ctx => ctx.exprIds.find?)
-    (fun ctx a b => { ctx with exprIds := ctx.exprIds.insert a b, exprIdsReverse := ctx.exprIdsReverse.push a})
-    fun ctx expr => pure ctx.exprIdsReverse.size
-
-def neutralCache (op : Nat) (var : Nat) : M (Option Expr) :=
-  lazyCache
-    (fun ctx => ctx.neutrals.find?)
-    (fun ctx a b => { ctx with neutrals := ctx.neutrals.insert a b })
-    (fun ctx (op, var) => do
-      let op := ctx.preContextsReverse[op].op
-      let var := ctx.exprIdsReverse[var]
-      getInstance ``IsNeutral #[op, var])
-    (op, var)
-
-inductive NormalizedExpr
-| maybeNormalized (opId : Nat) (l : NormalizedExpr) (r : NormalizedExpr)
-| definitelyNormalized (varId : Nat)
-| unnormalized (opId : Nat) (e : NormalizedExpr)
-  deriving Inhabited, Repr
-
-open NormalizedExpr
-
-def NormalizedExpr.norm : NormalizedExpr → M NormalizedExpr
-  | definitelyNormalized id => pure $ definitelyNormalized id
-  | e@(maybeNormalized opId _ _) => normalize opId e
-  | e@(unnormalized opId _) => normalize opId e
-where
-  loop (opId : Nat) : NormalizedExpr → StateT (Std.HashMap Nat (Option Expr)) M ACExpr
-      | definitelyNormalized x => do
-        let isNeutral ← neutralCache opId x
-        modify fun state => state.insert x isNeutral
-        return var x
-      | unnormalized _ e => loop opId e
-      | maybeNormalized _ l r => return op (←loop opId l) (←loop opId r)
-
-  normalize (opId : Nat) (e : NormalizedExpr) := do
-    let (orig, neutrals) ← loop opId e |>.run Std.HashMap.empty
-    let preContext := (←get).preContextsReverse[opId]
-    return convertBack opId $ evalList ACExpr preContext $ Lean.Data.AC.norm (neutrals, preContext) orig
-
-  convertBack (opId : Nat) : ACExpr → NormalizedExpr
-    | var id => definitelyNormalized id
-    | op l r => maybeNormalized opId (convertBack opId l) (convertBack opId r)
-
-def NormalizedExpr.decide : NormalizedExpr → M (Option (Nat × NormalizedExpr))
-  | definitelyNormalized _ => pure none
-  | unnormalized opId e => pure (opId, e)
-  | e@(maybeNormalized opId l r) => do
-    let rec loop : NormalizedExpr → StateT (Std.HashMap Nat (Option Expr)) M ACExpr
-      | definitelyNormalized x => do
-        let isNeutral ← neutralCache opId x
-        modify fun state => state.insert x isNeutral
-        return var x
-      | unnormalized _ e => loop e
-      | maybeNormalized _ l r => return op (←loop l) (←loop r)
-
-    let (orig, neutrals) ← loop e |>.run Std.HashMap.empty
-    let preContext := (←get).preContextsReverse[opId]
-    let res := evalList ACExpr preContext $ Lean.Data.AC.norm (neutrals, preContext) orig
-
-    return if orig == res then none else some (opId, e)
-
-open Lean.Expr
+inductive PreExpr
+| op (lhs rhs : PreExpr)
+| var (e : Expr)
 
 @[matchPattern] def bin {x₁ x₂} (op l r : Expr) :=
-  app (app op l x₁) r x₂
+  Expr.app (Expr.app op l x₁) r x₂
 
-@[matchPattern] def eq {eq₁ eq₂ eq₃ eq₄ app₁ app₂ n₁} (l r : Expr) :=
-  app (app (app (const (Lean.Name.str Lean.Name.anonymous "Eq" n₁) eq₁ eq₂) eq₃ eq₄) l app₁) r app₂
-
-partial def findUnnormalizedOperator (e : Expr) : M NormalizedExpr := do
-  match e with
-  | lam _ dom b _ => decide [dom, b] >>= wrap
-  | forallE _ dom b _ => decide [dom, b] >>= wrap
-  | letE _ ty val b _ => decide [ty, val, b] >>= wrap
-  | mdata _ e _ => findUnnormalizedOperator e
-  | proj _ _ e _ => decide [e] >>= wrap
-  | bin opExpr lExpr rExpr => do
-    match ←preContextCache opExpr with
-    | none => decide [lExpr, rExpr] >>= wrap
-    | some pc =>
-      match ←matchWithOp pc.id lExpr with
-      | (false, l) => return l
-      | (true, l) =>
-        match ←matchWithOp pc.id rExpr with
-        | (false, r) => return r
-        | (true, r) => return maybeNormalized pc.id l r
-
-  | app f a _ => decide [f, a] >>= wrap
-  | atom =>
-    return definitelyNormalized (←exprId atom)
-  where
-    decide : List Lean.Expr → M (Option (Nat × NormalizedExpr))
-    | [] => pure none
-    | x :: xs => do
-      match ←findUnnormalizedOperator x with
-      | definitelyNormalized _ => decide xs
-      | unnormalized opId e => pure $ some (opId, e)
-      | e@(maybeNormalized _ _ _) => return (←e.decide) <|> (←decide xs)
-
-    wrap : Option (Nat × NormalizedExpr) → M NormalizedExpr
-    | none => return definitelyNormalized (←exprId e)
-    | some (opId, e) => return unnormalized opId e
-
-    matchWithOp (op : Nat) (expr : Lean.Expr) : M (Bool × NormalizedExpr) := do
-      match ←findUnnormalizedOperator expr with
-      | e@(unnormalized _ _) => return (false, e)
-      | e@(definitelyNormalized _) =>
-        return (true, e)
-      | e@(maybeNormalized op₂ _ _) =>
-        match op == op₂ with
-        | true => return (true, e)
-        | false =>
-          match ←e.decide with
-          | none => return (true, definitelyNormalized (←exprId expr))
-          | some (op, e) => return (false, unnormalized op e)
-
-def buildProof (lhs rhs : NormalizedExpr) : M (Lean.Expr × Lean.Expr) := do
-  let vars :=
-    getVars (maybeNormalized 0 lhs rhs)
+def toACExpr (op l r : Expr) : MetaM (Array Expr × ACExpr) := do
+  let (preExpr, vars) ←
+    toPreExpr (mkApp2 op l r)
     |>.run Std.HashSet.empty
-    |>.2.toArray.insertionSort Nat.ble
-
+  let vars := vars.toArray.insertionSort Expr.lt
   let varMap := vars.foldl (fun xs x => xs.insert x xs.size) Std.HashMap.empty |>.find!
 
-  let (preContext, context) ← mkContext vars
-  let ty ← mkEq (←convertType preContext.op lhs) (←convertType preContext.op rhs) let lhs ← convert varMap lhs
-  let rhs ← convert varMap rhs
-  let proof ← mkAppM ``Context.eq_of_norm #[context, lhs, rhs, ←mkEqRefl $ ←mkAppM ``Lean.Data.AC.norm #[context, lhs]]
-  return (proof, ty)
+  return (vars, toACExpr varMap preExpr)
+  where
+    toPreExpr : Expr → StateT ExprSet MetaM PreExpr
+    | e@(bin op₂ l r) => do
+      if ←isDefEq op op₂ then
+        return PreExpr.op (←toPreExpr l) (←toPreExpr r)
+      modify fun vars => vars.insert e
+      return PreExpr.var e
+    | e => do
+      modify fun vars => vars.insert e
+      return PreExpr.var e
+
+    toACExpr (varMap : Expr → Nat) : PreExpr → ACExpr
+    | PreExpr.op l r => Data.AC.Expr.op (toACExpr varMap l) (toACExpr varMap r)
+    | PreExpr.var x => Data.AC.Expr.var (varMap x)
+
+def buildNormProof (preContext : PreContext) (l r : Expr) : MetaM (Lean.Expr × Lean.Expr) := do
+  let (vars, acExpr) ← toACExpr preContext.op l r
+
+  let (isNeutrals, context) ← mkContext vars
+  let acExprNormed := Data.AC.evalList ACExpr preContext $ Data.AC.norm (preContext, isNeutrals) acExpr
+  let tgt ← convertTarget vars acExprNormed
+  let lhs ← convert acExpr
+  let rhs ← convert acExprNormed
+  let α ← inferType vars[0]
+  let u ← getLevel α
+  let proof := mkAppN (mkConst ``Context.eq_of_norm [u.dec.get!]) #[α, context, lhs, rhs, ←mkEqRefl (mkConst ``Bool.true)]
+  return (proof, tgt)
 where
-  getVars : NormalizedExpr → StateM (Std.HashSet Nat) Unit
-    | definitelyNormalized x => modify fun xs => xs.insert x
-    | unnormalized opId e => getVars e
-    | maybeNormalized opId l r => do getVars l; getVars r
+  mkContext (vars : Array Expr) : MetaM (Array Bool × Expr) := do
+    let arbitrary := vars[0]
 
-  mkContext (vars : Array Nat) : M (PreContext × Lean.Expr) := do
-    let op :=
-      match lhs, rhs with
-      | definitelyNormalized _, definitelyNormalized _ => 0
-      | unnormalized opId _, _ => opId
-      | maybeNormalized opId _ _, _ => opId
-      | _, unnormalized opId _ => opId
-      | _, maybeNormalized opId _ _ => opId
-
-    let ctx ← get
-    let arbitrary := ctx.exprIdsReverse[vars[0]]
-    let preContext := ctx.preContextsReverse[op]
-    let vars : List Lean.Expr ← vars.toList.mapM fun x => do
-      let xExpr := ctx.exprIdsReverse[x]
+    let vars ← vars.mapM fun x => do
       let isNeutral ←
-        match ←neutralCache op x with
-        | none => mkAppOptM ``Option.none #[←mkAppM ``IsNeutral #[preContext.op, xExpr]]
-        | some isNeutral => mkAppM ``Option.some #[isNeutral]
+        match ←getInstance ``IsNeutral #[preContext.op, x] with
+        | none => pure (false, ←mkAppOptM ``Option.none #[←mkAppM ``IsNeutral #[preContext.op, x]])
+        | some isNeutral => pure (true, ←mkAppM ``Option.some #[isNeutral])
 
-      mkAppM ``Variable.mk #[xExpr, isNeutral]
+      return (isNeutral.1, ←mkAppM ``Variable.mk #[x, isNeutral.2])
 
-    let vars ← Lean.Meta.mkListLit (←mkAppM ``Variable #[preContext.op]) vars
+    let (isNeutrals, vars) := vars.unzip
+    let vars := vars.toList
+    let vars ← mkListLit (←mkAppM ``Variable #[preContext.op]) vars
 
     let comm ←
       match preContext.comm with
@@ -259,87 +120,51 @@ where
       match preContext.idem with
       | none => mkAppOptM ``Option.none #[←mkAppM ``IsIdempotent #[preContext.op]]
       | some idem => mkAppM ``Option.some #[idem]
-    return (preContext, ←mkAppM ``Lean.Data.AC.Context.mk #[preContext.op, preContext.assoc, comm, idem, vars, arbitrary])
 
-  convert (varMap : Nat → Nat) : NormalizedExpr → MetaM Lean.Expr
-    | definitelyNormalized id => mkAppM ``var #[Lean.mkNatLit $ varMap id]
-    | unnormalized _ e => convert varMap e
-    | maybeNormalized _ l r => do mkAppM ``op #[←convert varMap l, ←convert varMap r]
+    return (isNeutrals, ←mkAppM ``Lean.Data.AC.Context.mk #[preContext.op, preContext.assoc, comm, idem, vars, arbitrary])
 
-  convertType (op : Lean.Expr) : NormalizedExpr → M Lean.Expr
-    | definitelyNormalized id => do return (←get).exprIdsReverse[id]
-    | unnormalized _ e => convertType op e
-    | maybeNormalized _ l r => do mkAppM' op #[←convertType op l, ←convertType op r]
+  convert : ACExpr → MetaM Expr
+    | Data.AC.Expr.op l r => do mkAppM ``Data.AC.Expr.op #[←convert l, ←convert r]
+    | Data.AC.Expr.var x => mkAppM ``Data.AC.Expr.var #[mkNatLit x]
 
-inductive ProofStrategy
-  | ac_rfl (lhs rhs : NormalizedExpr)
-  | simp
-  | norm (e : NormalizedExpr)
+  convertTarget (vars : Array Expr) : ACExpr → MetaM Expr
+    | Data.AC.Expr.op l r => do mkAppM' preContext.op #[←convertTarget vars l, ←convertTarget vars r]
+    | Data.AC.Expr.var x => return vars[x]
 
-def pickStrategy (e : Expr) : M ProofStrategy := do
-  match e with
-  | eq l r =>
-    match ←findUnnormalizedOperator l with
-    | lhs@(unnormalized _ _) => return ProofStrategy.norm lhs
-    | lhs@(maybeNormalized _ _ _) =>
-      match ←findUnnormalizedOperator r with
-      | rhs@(unnormalized _ _) => return ProofStrategy.norm rhs
-      | rhs => return ProofStrategy.ac_rfl lhs rhs
-    | lhs@(definitelyNormalized _) =>
-      match ←findUnnormalizedOperator r with
-      | rhs@(unnormalized _ _) => return ProofStrategy.norm rhs
-      | rhs@(maybeNormalized _ _ _) => return ProofStrategy.ac_rfl lhs rhs
-      | rhs@(definitelyNormalized _) => return ProofStrategy.simp
-  | e => return ProofStrategy.norm $ ←findUnnormalizedOperator e
-
-def addAcEq (mvarId : MVarId) (e : NormalizedExpr) (target : Expr) : M MVarId := do
-  let (proof, ty) ← buildProof e (←e.norm)
-  let goal ← withLocalDeclD `h_ac ty fun h_ac =>
-    mkForallFVars #[h_ac] target
-  let goal ← mkFreshExprMVar goal
-  assignExprMVar mvarId (mkApp goal proof)
-  return goal.mvarId!
-
-partial def rewriteUnnormalized (mvarId : MVarId) : M Unit :=
-  withMVarContext mvarId do
-  let target ← getMVarType mvarId
-  match ←pickStrategy target with
-  | ProofStrategy.ac_rfl lhs rhs =>
-    trace[Meta.AC] "picking ac_rfl strategy {MessageData.ofGoal mvarId}"
-    try
-      let (proof, ty) ← buildProof lhs rhs
-      if ←isDefEq target ty then
-        assignExprMVar mvarId proof
-      else throwError ""
-    catch _ => throwError "cannot synthesize proof:\n{MessageData.ofGoal mvarId}"
-  | ProofStrategy.simp =>
-    trace[Meta.AC] "picking simp strategy {MessageData.ofGoal mvarId}"
-    let simpCtx ← Simp.Context.mkDefault
-    let newGoal ← simpTarget mvarId simpCtx
-    unless newGoal.isNone do
-      throwError "cannot synthesize proof:\n{MessageData.ofGoal mvarId}"
-  | ProofStrategy.norm (definitelyNormalized _) => throwError "no unnormalized operators found"
-  | ProofStrategy.norm e =>
-    trace[Meta.AC] "picking norm strategy {MessageData.ofGoal mvarId}"
-    let mvarId ← addAcEq mvarId e target
-    let (h_ac, mvarId) ← intro mvarId `h_ac
-    let simpCtx ← Simp.Context.mkDefault
-    withMVarContext mvarId do
-    let simpCtx := { simpCtx with simpTheorems := ←simpCtx.simpTheorems.add #[] (mkFVar h_ac) }
-
-    trace[Meta.AC] "pre rewrite state:\n{MessageData.ofGoal mvarId}\n"
-    let mvarId ← simpTarget mvarId simpCtx
-    if let some mvarId := mvarId then
-      if not $ ←isDefEq target (←getMVarType mvarId) then
-        let mvarId ← clear mvarId h_ac
-        trace[Meta.AC] "post rewrite state:\n{MessageData.ofGoal mvarId}\n"
-        rewriteUnnormalized mvarId
-      else
-        throwError "cannot synthesize proof:\n{MessageData.ofGoal mvarId}"
+def rewriteUnnormalized (mvarId : MVarId) : MetaM Unit := do
+  let simpCtx :=
+    {
+      simpTheorems  := {}
+      congrTheorems := (← getSimpCongrTheorems)
+      config        := Simp.neutralConfig
+    }
+  let tgt ← getMVarType mvarId
+  let res ← Simp.main tgt simpCtx (methods := { post })
+  let newGoal ← applySimpResultToTarget mvarId tgt res
+  applyRefl newGoal
+where
+  post (e : Expr) : SimpM Simp.Step := do
+    let ctx ← read
+    match e, ctx.parent? with
+    | bin op₁ l r, some (bin op₂ _ _) =>
+      if ←isDefEq op₁ op₂ then
+        return Simp.Step.done { expr := e }
+      match ←preContext op₁ with
+      | some pc =>
+        let (proof, newTgt) ← buildNormProof pc l r
+        return Simp.Step.done { expr := newTgt, proof? := proof }
+      | none => return Simp.Step.done { expr := e }
+    | bin op l r, none =>
+      match ←preContext op with
+      | some pc =>
+        let (proof, newTgt) ← buildNormProof pc l r
+        return Simp.Step.done { expr := newTgt, proof? := proof }
+      | none => return Simp.Step.done { expr := e }
+    | e, _ => return Simp.Step.done { expr := e }
 
 @[builtinTactic ac_refl] def ac_refl_tactic : Lean.Elab.Tactic.Tactic := fun stx => do
   let goal ← getMainGoal
-  (rewriteUnnormalized goal).run' emptyACNormContext
+  rewriteUnnormalized goal
 
 builtin_initialize
   registerTraceClass `Meta.AC
